More progress towards const prop.

theories/ValueOpts/ConstantPropagation.v
@@ -104,14 +104,14 @@ Inductive cp_sound : onv (withTop val)
 | CPIf AE Cp Rch e (b:bool) s1 s2 (r1 r2:ann bool)
        (Cond1:cp_sound AE Cp Rch s1 r1)
        (Cond2:cp_sound AE Cp Rch s2 r2)
-       (Reach1:b -> aval2bool (op_eval AE e) <> None -> aval2bool (op_eval AE e) <> (Some false) -> getAnn r1)
-       (Reach2:b -> aval2bool (op_eval AE e) <> None -> aval2bool (op_eval AE e) <> (Some true) -> getAnn r2)
+       (Reach1:b -> op_eval AE e <> None -> aval2bool (op_eval AE e) <> Some false -> getAnn r1)
+       (Reach2:b -> poLe (Some (wTA val_false)) (op_eval AE e) -> getAnn r2)
   : cp_sound AE Cp Rch (stmtIf e s1 s2) (ann2 b r1 r2)
 | CPGoto AE l Y Cp Rch Z aY (b bf:bool)
   : get Cp (counted l) (Z,aY)
     -> get Rch (counted l) bf
     -> length Z = length Y
-    -> (b -> PIR2 (@poLe _ (PartialOrder_option _)) (List.map (op_eval AE) Y) aY)
+    -> (b -> PIR2 poLe (List.map (op_eval AE) Y) aY)
     -> (b -> bf)
     -> cp_sound AE Cp Rch (stmtApp l Y) (ann0 b)
 | CPReturn AE Cp Rch e b
@@ -151,13 +151,14 @@ Proof.
         decide (a -> getAnn r); try dec_solve.
   - edestruct (IH s2 ltac:(eauto) AE Rch ZL); eauto; [| dec_solve];
       edestruct (IH s1 ltac:(eauto) AE Rch ZL); eauto; [| dec_solve];
-    decide (aval2bool (op_eval AE e) = Some false);
-    (decide (aval2bool (op_eval AE e) = Some true));
-    decide (a); decide (getAnn r1); decide (getAnn r2); try dec_solve.
+        decide (op_eval AE e = None);
+        decide (aval2bool (op_eval AE e) = Some false);
+        (decide (poLe (Some (wTA val_false)) (op_eval AE e)));
+        decide (a); decide (getAnn r1); decide (getAnn r2); try dec_solve.
   - destruct (get_dec ZL (counted l)) as [[[]]|]; try dec_solve.
     destruct (get_dec Rch (counted l)) as [[]|]; try dec_solve.
     decide (length l0 = length Y); try dec_solve.
-    decide (a -> PIR2 (@poLe _ (PartialOrder_option _)) (List.map (op_eval AE) Y) l1);
+    decide (a -> PIR2 poLe (List.map (op_eval AE) Y) l1);
       try dec_solve.
     decide (a -> x); try dec_solve.
   - assert (SZ:size s < size (stmtFun F s)) by eauto.
@@ -171,8 +172,9 @@ Defined.
 
 Definition cp_eqn (E:onv (withTop val)) x :=
   match E x with
-    | Some (wTA c) => singleton (EqnEq (Var x) (Con c))
-    | _ => ∅
+  | Some (wTA c) => singleton (EqnEq (Var x) (Con c))
+  | None => singleton EqnBot
+  | _ => ∅
   end.
 
 Instance cp_eqn_eq E
@@ -342,6 +344,34 @@ Proof.
   hnf in SAT; simpl in *. inv SAT; eauto.
 Qed.
 
+Lemma in_cp_eqns_bot AE x lv
+  : x \In lv
+    -> AE x = ⎣⎦
+    -> EqnBot ∈ cp_eqns AE lv.
+Proof.
+  intros. unfold cp_eqns.
+  eapply fold_union_incl.
+  instantiate (1:=singleton EqnBot).
+  cset_tac; intuition.
+  assert (cp_eqn AE x = singleton EqnBot).
+  unfold cp_eqn. rewrite H0. reflexivity.
+  rewrite <- H1. eapply map_1; eauto.
+  eauto with typeclass_instances.
+Qed.
+
+Lemma cp_eqns_satisfies_env_none AE E x lv
+: x ∈ lv
+  -> AE x = None
+  -> satisfiesAll E (cp_eqns AE lv)
+  -> E x = None.
+Proof.
+  intros. exploit H1 as SAT; eauto.
+  instantiate (1:=EqnBot).
+  eapply in_cp_eqns_bot; eauto.
+  hnf in SAT; simpl in *. inv SAT; eauto.
+Qed.
+
+
 Ltac smatch :=
   match goal with
     | [ H : match ?x with
@@ -363,23 +393,37 @@ Lemma op_eval_same e lv AE E v
 :   Op.freeVars e ⊆ lv
     -> op_eval AE e = Some (wTA v)
     -> satisfiesAll E (cp_eqns AE lv)
-    -> exists v', Op.op_eval E e = Some v' /\ option_eq eq ⎣v' ⎦ ⎣v ⎦.
+    -> Op.op_eval E e = Some v.
 Proof.
   intros. general induction e; simpl in * |- *; eauto 20 using @option_eq.
   - exploit cp_eqns_satisfies_env; eauto using @option_eq.
     + cset_tac.
   - repeat imatch.
-    edestruct IHe; eauto; dcr.
-    rewrite H5; simpl.
-    eexists; split; eauto using @option_eq.
-    inv H6; eauto.
+    erewrite IHe; eauto; dcr.
   - repeat imatch.
-    edestruct IHe1; eauto. cset_tac; intuition.
-    edestruct IHe2; eauto. cset_tac; intuition.
-    dcr.
-    rewrite H6, H7; simpl.
-    inv H8; inv H9.
-    eexists v; split; eauto using @option_eq.
+    erewrite IHe1; eauto.
+    erewrite IHe2; eauto.
+    cset_tac. cset_tac.
+Qed.
+
+Lemma op_eval_None e lv AE E
+:   Op.freeVars e ⊆ lv
+    -> op_eval AE e = None
+    -> satisfiesAll E (cp_eqns AE lv)
+    -> Op.op_eval E e = None.
+Proof.
+  intros. general induction e; simpl in * |- *; eauto 20 using @option_eq.
+  - exploit cp_eqns_satisfies_env_none; eauto using @option_eq.
+    + cset_tac.
+  - repeat imatch.
+    + erewrite op_eval_same; eauto; dcr; subst.
+    + erewrite IHe; eauto; dcr.
+  - repeat imatch.
+    + erewrite !op_eval_same; eauto; cset_tac.
+    + erewrite op_eval_same; eauto.
+      erewrite IHe2; eauto.
+      cset_tac. cset_tac.
+    + erewrite IHe1; eauto. cset_tac.
 Qed.
 
 Lemma op_eval_entails AE e v x lv
@@ -420,11 +464,9 @@ Proof.
   unfold cp_choose_op. case_eq (op_eval AE e); try destruct w; intros.
   - eapply entails_eqns_apx_refl.
   - hnf; intros.
-    case_eq (Op.op_eval E e); intros; simpl.
-    + edestruct op_eval_same; try eapply H1; eauto; dcr.
-      hnf; intros. cset_tac'. rewrite <- H3; simpl.
-      rewrite H4. inv H5. reflexivity.
-    + edestruct op_eval_same; try eapply H1; eauto; dcr. congruence.
+    eapply op_eval_same in H; eauto.
+    hnf; intros. cset_tac'. rewrite <- H2; simpl.
+    rewrite H.  reflexivity.
   - eapply entails_eqns_apx_refl.
 Qed.
 
@@ -513,79 +555,98 @@ Proof.
     + destruct a0.
       * cset_tac'. hnf in H4; subst; simpl in *.
         rewrite H0 in H1. cset_tac.
-  - rewrite H in H4. isabsurd.
+  - rewrite H in H4. cset_tac'.
+    rewrite <- H4 in H0. simpl in *.
+    exfalso. rewrite H0 in H1. cset_tac.
 Qed.
 
 Lemma in_subst_eqns gamma Z Y AE
 : length Z = length Y
   -> gamma \In subst_eqns (sid [Z <-- Y]) (cp_eqns AE (of_list Z))
-  -> exists n x c,
+  -> (exists n x c,
       gamma = subst_eqn (sid [Z <-- Y]) (EqnEq (Var x) (Con c))
       /\ AE x = Some (wTA c)
       /\ get Z n x
-      /\ get Y n ((sid [Z <-- Y]) x).
+      /\ get Y n ((sid [Z <-- Y]) x))
+    \/ (exists n x,
+      gamma = subst_eqn (sid [Z <-- Y]) (EqnBot)
+      /\ AE x = None
+      /\ EqnBot ∈ cp_eqns AE (of_list Z)
+      /\ get Z n x
+      /\ get Y n ((sid [Z <-- Y]) x)).
 Proof.
   intros.
   edestruct subst_eqns_in as [γ' ?]; eauto; dcr; subst.
   edestruct cp_eqns_in as [x ?]; eauto; dcr.
   unfold cp_eqn in H4. case_eq (AE x); intros.
-  - rewrite H1 in H4. destruct w; isabsurd.
+  - left. rewrite H1 in H4. destruct w; isabsurd.
     destruct a; isabsurd.
     cset_tac'. invc H4.
     unfold subst_eqn; simpl.
     edestruct (update_with_list_lookup_in_list sid Z Y) as [? [? ]]; eauto; dcr.
     invc H9. invc H7.
     eexists x0, x2; repeat split; eauto.
-  - exfalso. rewrite H1 in H4; isabsurd.
+  - right. rewrite H1 in H4.
+    cset_tac'. invc H4.
+    unfold subst_eqn; simpl.
+    edestruct (update_with_list_lookup_in_list sid Z Y) as [? [? ]]; eauto; dcr.
+    invc H9. invc H7.
+    eexists x0, x2; repeat split; eauto.
 Qed.
-
-Lemma entails_cp_eqns_subst AE D Z Y
-: length Z = length Y
-  -> PIR2 (@poLe _ (PartialOrder_option _))
-         (List.map (op_eval AE) Y) (lookup_list AE Z)
-  -> list_union (List.map Op.freeVars Y)[<=]D
-  -> entails (cp_eqns AE D)
-            (subst_eqns (sid [Z <-- Y]) (cp_eqns AE (of_list Z))).
-Proof.
-  intros LEQ le_prec INCL.
-  hnf. intros. hnf. intros.
-
-  edestruct in_subst_eqns as [? [? []]]; eauto; dcr.
-  edestruct PIR2_nth_2; eauto; dcr.
-  - rewrite lookup_list_map.
-    eapply map_get_1. eauto.
-  - inv_get.
-    rewrite H4 in H7; simpl in *; clear_trivial_eqs.
-    edestruct op_eval_same; eauto; dcr; clear_trivial_eqs.
-    + rewrite <- INCL.
-      eapply incl_list_union. eapply map_get_1; eauto. reflexivity.
-    + rewrite <- H5. reflexivity.
-Qed.
-
 
 Lemma entails_cp_eqns_subst_choose AE AE' D Z Y
 : length Z = length Y
-  -> PIR2 (@poLe _ (PartialOrder_option _)) (List.map (op_eval AE) Y) (lookup_list AE' Z)
+  -> PIR2 poLe (List.map (op_eval AE) Y) (lookup_list AE' Z)
   -> list_union (List.map Op.freeVars Y)[<=]D
-  -> entails (cp_eqns AE D)
+  -> entails (of_list ((fun y => EqnEq y y) ⊝ cp_choose_op AE ⊝ Y) ∪ cp_eqns AE D)
             (subst_eqns (sid [Z <-- List.map (cp_choose_op AE) Y])
                         (cp_eqns AE' (of_list Z))).
 Proof.
   intros LEQ le_prec INCL.
   hnf. intros. hnf. intros.
 
-  edestruct in_subst_eqns as [? [? []]]; try eapply H0; eauto with len; dcr; subst.
-  edestruct map_get_4; eauto; dcr.
-  edestruct PIR2_nth_2; eauto; dcr.
-  rewrite lookup_list_map.
-  eapply map_get_1. eauto. rewrite H4 in *; simpl in *.
-  clear_trivial_eqs.
-  edestruct op_eval_same; eauto; dcr.
-  + rewrite <- INCL.
-    eapply incl_list_union. eapply map_get_1; eauto. reflexivity.
-  + hnf; simpl. inv_get. reflexivity.
-  + hnf. simpl. rewrite <- H2.
-    unfold cp_choose_op. inv_get. simpl. reflexivity.
+  edestruct in_subst_eqns as [[? [? []]]|]; try eapply H0; eauto with len; dcr; subst.
+  - inv_get.
+    edestruct PIR2_nth_2; eauto; dcr.
+    + rewrite lookup_list_map.
+      eapply map_get_1. eauto.
+    + rewrite H4 in *; simpl in *.
+      clear_trivial_eqs. inv_get.
+      exploit H. instantiate (1:=EqnEq (cp_choose_op AE x2) (cp_choose_op AE x2)).
+      eapply incl_left. eapply get_in_of_list.
+      eapply map_get_eq; eauto. inv H1; subst.
+      inv H5; clear_trivial_eqs.
+      * exfalso. exploit op_eval_None; eauto.
+        instantiate (1:=D).
+        erewrite <- INCL.
+        eapply incl_list_union. eapply map_get_1; eauto. reflexivity.
+        hnf; intros. eapply H. cset_tac. unfold cp_choose_op in H2. rewrite <- H9 in H2.
+        congruence.
+      * exploit op_eval_same; eauto; dcr.
+        -- instantiate (1:=D).
+           rewrite <- INCL.
+           eapply incl_list_union. eapply map_get_1; eauto. reflexivity.
+        -- hnf; intros. eapply H. cset_tac.
+        -- rewrite <- EQ.
+           unfold cp_choose_op. rewrite <- H7. simpl.
+           econstructor; eauto.
+  - simpl. inv_get.
+    simpl in *.
+    edestruct PIR2_nth_2; eauto; dcr.
+    + rewrite lookup_list_map.
+      eapply map_get_1. eauto.
+    + rewrite H3 in *. inv H6.
+      inv_get.
+      exploit H.
+      instantiate (1:=EqnEq (cp_choose_op AE x1) (cp_choose_op AE x1)).
+      eapply incl_left. eapply get_in_of_list.
+      eapply map_get_eq; eauto. inv H1; subst.
+      exploit op_eval_None; eauto.
+      instantiate (1:=D).
+      erewrite <- INCL.
+      eapply incl_list_union. eapply map_get_1; eauto. reflexivity.
+      hnf; intros. eapply H. cset_tac. unfold cp_choose_op in H6.
+      rewrite <- H2 in *. congruence.
 Qed.
 
 Lemma cp_eqns_update D x c AE
@@ -622,10 +683,25 @@ Proof.
   case_eq (op_eval AE e); intros.
   - rewrite H1 in H; eauto.
     simpl in *. destruct w; isabsurd.
-    edestruct op_eval_same; eauto; dcr.
+    exploit op_eval_same; eauto; dcr.
     clear_trivial_eqs. eauto.
   - rewrite H1 in H. inv H.
 Qed.
+
+(*
+Lemma aval2bool_none AE e lv (FV:Op.freeVars e [<=] lv)
+  : aval2bool (op_eval AE e) = None
+    -> forall E, satisfiesAll E (cp_eqns AE lv) -> Op.op_eval E e = None.
+Proof.
+  intros.
+  case_eq (op_eval AE e); intros.
+  - rewrite H1 in H; eauto.
+    simpl in *. destruct w; isabsurd.
+    exploit op_eval_same; eauto; dcr.
+    clear_trivial_eqs. eauto.
+  - rewrite H1 in H. inv H.
+Qed.
+ *)
 
 Lemma satisfies_BinOpEq_inv_true E e e'
   : satisfies E (EqnEq (UnOp UnOpToBool (BinOp BinOpEq e e')) (Con val_true))
@@ -637,7 +713,7 @@ Proof.
   simpl in *. inv H.
   pose proof (Integers.Int.eq_spec v v0).
   destruct (Integers.Int.eq v v0); intros; isabsurd.
-  subst; eauto. reflexivity.
+  subst; eauto. econstructor; eauto.
 Qed.
 
 Lemma satisfies_UnOpToBool_inv_false E e
@@ -648,7 +724,7 @@ Proof.
   destruct (Op.op_eval E e); isabsurd.
   simpl in *. inv H.
   unfold val2bool in H2. cases in H2.
-  - reflexivity.
+  - econstructor. reflexivity.
   - simpl in *. isabsurd.
 Qed.
 
@@ -735,11 +811,18 @@ Proof.
            eapply entails_union; split.
            unfold cp_eqn.
            case_eq (AE x); intros; eauto using entails_empty.
-           rewrite H1 in H. exploit H; eauto. inv H2.
-           repeat cases; eauto using entails_empty.
-           eapply op_eval_entails; eauto.
-           eapply entails_monotone. reflexivity.
-           cset_tac.
+           ++ rewrite H1 in H. exploit H; eauto. inv H2.
+             repeat cases; eauto using entails_empty.
+             eapply op_eval_entails; eauto.
+           ++ simpl in *. hnf; intros.
+             exfalso. exploit H2.
+             instantiate (1:=EqnEq (Var x) (cp_choose_op AE e)). cset_tac.
+             unfold cp_choose_op in H3.
+             rewrite H in H3; eauto. rewrite H1 in H3.
+             simpl in H3. rewrite H1 in H.
+             erewrite op_eval_None in H3; eauto.
+             inv H3. hnf; intros. eapply H2. cset_tac.
+           ++ eapply entails_subset. cset_tac.
         -- eapply entails_bot. cset_tac.
         -- eapply entails_bot. cset_tac.
       * cases.
@@ -755,7 +838,8 @@ Proof.
            case_eq (AE x); intros; eauto using entails_empty.
            rewrite H1 in H. exploit H; eauto. inv H2.
            repeat cases; eauto using entails_empty.
-        -- reflexivity.
+           simpl in *. exploit H; eauto. congruence.
+        -- eapply entails_subset. cset_tac.
         -- eapply entails_bot. cset_tac.
         -- eapply entails_bot. cset_tac.
       * cases.
@@ -778,13 +862,22 @@ Proof.
             edestruct aval2bool_inv_val; eauto; dcr.
             assert (w = x) by congruence; subst.
             rewrite H12. simpl. eapply val_false_true_neq.
-          + decide (aval2bool (op_eval AE e) = None).
-            *
+          + decide (op_eval AE e = None).
+            * decide (getAnn r1).
+              -- eapply eqn_sound_entails_monotone; eauto.
+                 cases. pe_rewrite. eapply entails_subset. cset_tac.
+              -- eapply eqn_sound_entails_monotone; eauto.
+                 cases; eauto.
+                 hnf; intros. exfalso.
+                 exploit H. instantiate (1:=EqnEq (UnOp UnOpToBool e) (Con val_true)).
+                 cset_tac. simpl in H0.
+                 erewrite op_eval_None in H0; eauto. simpl in *.
+                 inv H0.
+                 hnf; intros. eapply H. cset_tac.
             * eapply eqn_sound_entails_monotone; eauto.
+              exploit Reach1; eauto.
               cases.
-              -- pe_rewrite. eapply entails_add''. reflexivity.
-              -- exfalso. eapply Reach1; eauto.
-
+              pe_rewrite. eapply entails_add''. reflexivity.
         - eapply eqn_sound_entails_monotone; eauto.
           eapply entails_bot. cset_tac.
       }
@@ -797,10 +890,28 @@ Proof.
            edestruct aval2bool_inv_val; eauto; dcr.
            assert (w = x) by congruence; subst.
            rewrite H12. eapply val_true_false_neq.
-          + eapply eqn_sound_entails_monotone; eauto.
-            cases.
-            * pe_rewrite. eapply entails_add''. reflexivity.
-            * exfalso. eapply Reach2; eauto.
+          + decide (op_eval AE e = None).
+            * decide (getAnn r2).
+              -- eapply eqn_sound_entails_monotone; eauto.
+                 cases. pe_rewrite. eapply entails_subset. cset_tac.
+              -- eapply eqn_sound_entails_monotone; eauto.
+                 cases; eauto.
+                 hnf; intros. exfalso.
+                 exploit H. instantiate (1:=EqnEq (UnOp UnOpToBool e) (Con val_false)).
+                 cset_tac. simpl in H0.
+                 erewrite op_eval_None in H0; eauto. simpl in *.
+                 inv H0.
+                 hnf; intros. eapply H. cset_tac.
+            * exploit Reach2; eauto.
+              revert n.
+              case_eq(op_eval AE e); intros; try congruence.
+              simpl in *. destruct w; simpl in *.
+              -- econstructor; eauto. econstructor.
+              -- unfold val2bool in n. cases in n; isabsurd.
+                 econstructor; reflexivity.
+              -- eapply eqn_sound_entails_monotone; eauto.
+                 cases. pe_rewrite.
+                 eapply entails_subset; eauto. cset_tac.
         - eapply eqn_sound_entails_monotone; eauto.
           eapply entails_bot. cset_tac.
       }
@@ -815,7 +926,9 @@ Proof.
       * rewrite H13. cases.
         eapply entails_cp_eqns_subst_choose; eauto.
 
-      * eapply entails_bot; eauto.
+
+
+      * eapply entails_bot; eauto. cset_tac.
     + cases.
       * eapply cp_choose_approx_list; eauto.
       * eapply entails_bot; eauto.
@@ -884,7 +997,7 @@ Require Import CMap.
 
 Lemma cp_eqns_no_assumption d G
 : (forall x : var,
-   x \In G -> MapInterface.find x d = ⎣⎦)
+   x \In G -> MapInterface.find x d = ⎣Top⎦)
    -> cp_eqns (fun x0 : var => MapInterface.find x0 d) G [=] ∅.
 Proof.
   intros. revert H. pattern G. eapply set_induction.
